Semantic weakening

ERTLeanTogether/ERTLeanTogether/StlcDeBruijn.lean
@@ -1,18 +1,30 @@
 namespace StlcDeBruijn
 
 inductive Ty
+| unit
 | nat
 | fn (A B: Ty)
 
 open Ty
 
+def Ty.den: Ty -> Type
+| unit => Unit
+| nat => Nat
+| fn A B => A.den -> Option (B.den)
+
 def Ctx := List Ty
+
+inductive Ctx.den: Ctx -> Type
+| nil: Ctx.den []
+| cons: Option (Ty.den A) -> Ctx.den Γ -> Ctx.den (A::Γ)
 
 inductive Stlc: Type
 | var (n: Nat)
 | app (s t: Stlc)
 | lam (A: Ty) (t: Stlc)
+| nil
 | cnst (n: Nat)
+| abort (A: Ty)
 
 def liftWk (ρ: Nat -> Nat): Nat -> Nat
 | 0 => 0
@@ -50,13 +62,17 @@ inductive HasTy : Ctx -> Stlc -> Ty -> Type
     -> HasTy Γ t A
     -> HasTy Γ (app s t) B
 | lam : HasTy (A :: Γ) t B -> HasTy Γ (lam A t) (fn A B)
+| nil: HasTy Γ nil unit
 | cnst : HasTy Γ (cnst n) nat
+| abort: HasTy Γ (abort A) A
 
 theorem HasTy.ty_coh: HasTy Γ s A -> HasTy Γ s B -> A = B
 | var v, var v' => Var.ty_coh v v'
 | app s _, app s' _ => by cases (ty_coh s s'); rfl
 | lam t, lam t' => by rw [ty_coh t t']
+| nil, nil => rfl
 | cnst, cnst => rfl
+| abort, abort => rfl
 
 theorem HasTy.coh: (h h': HasTy Γ s A) -> h = h'
 | var v, var v' => by rw [Var.coh v v']
@@ -64,7 +80,9 @@ theorem HasTy.coh: (h h': HasTy Γ s A) -> h = h'
   cases (ty_coh s s')
   rw [coh s s', coh t t']
 | lam t, lam t' => by rw [coh t t']
+| nil, nil => rfl
 | cnst, cnst => rfl
+| abort, abort => rfl
 
 open HasTy
 
@@ -84,7 +102,9 @@ def HasTy.wk (R: Wk ρ Γ Δ): HasTy Δ s A -> HasTy Γ (wk ρ s) A
 | var v => var (v.wk R)
 | app s t => app (wk R s) (wk R t)
 | lam t => lam (wk R.lift t)
+| nil => nil
 | cnst => cnst
+| abort => abort
 
 def liftSubst (σ: Nat -> Stlc) : Nat -> Stlc
 | 0 => var 0
@@ -114,4 +134,39 @@ def HasTy.subst (S: Subst σ Γ Δ): HasTy Δ s A
 | var v => S v
 | app s t => app (subst S s) (subst S t)
 | lam t => lam (subst S.lift t)
+| nil => nil
 | cnst => cnst
+| abort => abort
+
+def Var.den: Var Γ n A -> Ctx.den Γ -> Option A.den
+| head, Ctx.den.cons a _ => a
+| tail v, Ctx.den.cons _ G => v.den G
+
+def HasTy.den: HasTy Γ s A -> Ctx.den Γ -> Option A.den
+| var v, G => v.den G
+| app s t, G => do
+  let s <- s.den G
+  let t <- t.den G
+  s t
+| lam t, G => pure (λx => t.den (Ctx.den.cons x G))
+| nil, G => pure ()
+| @cnst _ n, _ => pure n
+| abort, _ => none
+
+def Wk.den: Wk ρ Γ Δ -> Ctx.den Γ -> Ctx.den Δ
+| nil, x => x
+| lift ρ, Ctx.den.cons a G => Ctx.den.cons a (ρ.den G)
+| step ρ, Ctx.den.cons a G => ρ.den G
+
+theorem Var.wk_den: (v: Var Δ n A) -> (R: Wk ρ Γ Δ)
+  -> ∀{G: Γ.den}, v.den (R.den G) = (v.wk R).den G
+| head, lift R, Ctx.den.cons _ _ => rfl
+| tail v, lift R, Ctx.den.cons _ _
+| v, step R, Ctx.den.cons _ _ => by simp [Wk.den, den, v.wk_den R]
+
+theorem HasTy.wk_den (R: Wk ρ Γ Δ) (h: HasTy Δ a A)
+  : ∀{G: Γ.den}, h.den (R.den G) = (h.wk R).den G := by
+  induction h generalizing ρ Γ with
+  | var v => exact Var.wk_den v R
+  | lam t I => intros; simp [den, <-I]; rfl
+  | _ => simp [den, *]
