ERTLeanTogether/ERTLeanTogether/StlcIntrinsic.lean
@@ -1,7 +1,7 @@
 namespace StlcIntrinsic
 
 inductive Ty
-| unit
+| nat
 | fn (A B: Ty)
 
 def Ctx := List Ty
@@ -10,13 +10,18 @@ inductive Var: Ctx -> Ty -> Type
 | head: Var (A :: Γ) A
 | tail: Var Γ A -> Var (B :: Γ) A
 
+def Ty.den: Ty -> Type
+| nat => Nat
+| fn A B => A.den -> Option (B.den)
+
 open Var
 
 inductive Stlc: Ctx -> Ty -> Type
 | var: Var Γ A -> Stlc Γ A
 | app: Stlc Γ (Ty.fn A B) -> Stlc Γ A -> Stlc Γ B
 | lam: Stlc (A :: Γ) B -> Stlc Γ (Ty.fn A B)
-| unit: Stlc Γ Ty.unit
+| cnst: Nat -> Stlc Γ Ty.nat
+| abort: Stlc Γ A
 
 open Stlc
 
@@ -36,4 +41,5 @@ def Stlc.wk (ρ: Wk Γ Δ): Stlc Δ A -> Stlc Γ A
 | var v => var (v.wk ρ)
 | app s t => app (s.wk ρ) (t.wk ρ)
 | lam s => lam (s.wk ρ.lift)
-| unit => unit
+| cnst n => cnst n
+| abort => abort
